change semantics, add accumulator example

src/ocaml/parser/ast.ml
@@ -6,6 +6,7 @@ type size = Z.t
 type fgtyp =
   Tuint of size
 | Tsint of size
+| Clock
 
 let uint_t w = Tuint w
 let int_t w = Tsint w
@@ -54,10 +55,10 @@ type ebinop =
 
 type fexpr =
   | Econst of int
-  | Evar of var
-  | Eref of var * fgtyp
-  | Efield of var * fexpr
-  | Esubacc of var * Z.t
+  | Eref of var
+  | Edeclare of var * fgtyp
+  (* | Efield of var * fexpr
+  | Esubacc of var * Z.t *)
   | Eprim_unop of eunop * fexpr
   | Eprim_binop of ebinop * fexpr * fexpr
   | Emux of fexpr * fexpr * fexpr
@@ -79,13 +80,21 @@ type fmem =
     read_write : ruw
   }
 
+type rst =
+  | NRst 
+  | Rst of fexpr * fexpr
+
+  
 type freg =
   {
     rid : var;
-    rtype : fexpr;
-    reset : fexpr list
+    rtype : fgtyp;
+    clock : fexpr;
+    reset : rst
   }
 
+let mkfreg v t c e1 e2 = { rid = v; rtype = t; clock = c; reset = Rst (e1, e2) }
+  
 type fstmt =
   | Sskip
   | Swire of var * fgtyp
@@ -96,7 +105,7 @@ type fstmt =
   | Sfcnct of fexpr * fexpr
   | Spcnct of fexpr * fexpr
   | Sinvalid of var
-  | Sattach of var list
+  (*  | Sattach of var list *)
   | Swhen of fexpr * fstmt * fstmt
   | Sstop of fexpr * fexpr * Z.t
   | Sprintf (* TBD *)
@@ -106,8 +115,8 @@ type fstmt =
   | Sparam of var * fexpr (* TBD *)
 
 type fport =
-  | Finput of fexpr
-  | Foutput of fexpr
+  | Finput of var * fgtyp
+  | Foutput of var * fgtyp
 
 type fmodule =
   | FInmod of var * fport list * fstmt list
@@ -122,6 +131,7 @@ let pp_type out ty =
   match ty with
   | Tuint s -> output_string out "(Tunit "; output_string out (Z.to_string s); output_string out ")"
   | Tsint s -> output_string out "(Tsnit "; output_string out (Z.to_string s); output_string out ")"
+  | Clock -> output_string out "Clock"
           
 let pp_unop out op =
   match op with
@@ -135,8 +145,8 @@ let pp_binop out op =
           
 let rec pp_expr out e =
   match e with
-  | Evar v -> output_string out "(Evar "; output_string out (v^" "); output_string out ")"
-  | Eref (v, ty) -> output_string out "(Eref "; output_string out (v^" "); output_string out " "; pp_type out ty; output_string out ")\n"
+  | Eref v -> output_string out "(Eref "; output_string out (v^" "); output_string out ")"
+  | Edeclare (v, ty) -> output_string out "(Edeclare "; output_string out (v^" "); output_string out " "; pp_type out ty; output_string out ")\n"
   | Eprim_unop (op, e1) -> output_string out "(Eprim_unop "; pp_unop out op; pp_expr out e1; output_string out ")"
   | Eprim_binop (bop, e1, e2) -> output_string out "(Eprim_binop "; pp_binop out bop; pp_expr out e1; output_string out " "; pp_expr out e2; output_string out ")"
   | _ -> output_string out ""
@@ -147,10 +157,10 @@ let rec pp_ports out pl =  List.iter (fun c -> pp_port out c; output_string out 
                      
 and pp_port out p =
   match p with
-  | Finput e -> output_string out "(Finput "; pp_expr out e; output_string out ")\n"
-  | Foutput e -> output_string out "(Foutput "; pp_expr out e; output_string out ")\n"                 
+  | Finput (v, ty) -> output_string out "(Finput "; output_string out (v^" "); pp_type out ty; output_string out ")\n"
+  | Foutput (v, ty) -> output_string out "(Foutput "; output_string out (v^" "); pp_type out ty; output_string out ")\n"                 
                  
-
+                       
 let rec pp_statements out sl = List.iter (fun c -> pp_statement out c; output_string out "") sl
                              
 and  pp_statement out s =
@@ -160,18 +170,24 @@ and  pp_statement out s =
   | Sfcnct (e1, e2) -> output_string out "(Sfcnct "; pp_expr out e1; output_string out " "; pp_expr out e2; output_string out ")\n"
   | Spcnct (e1, e2) -> output_string out "(Spcnct "; pp_expr out e1; output_string out " "; pp_expr out e2; output_string out ")\n"
   | Swhen (e, s1, s2) -> output_string out "(Swhen "; pp_expr out e; pp_statement out s1; pp_statement out s2; output_string out ")\n"
+  | Sreg r ->
+     (match r.reset with
+     | NRst -> output_string out "Sreg (mk_freg ("; output_string out ((r.rid)^" "); pp_type out (r.rtype); output_string out " "; pp_expr out (r.clock); output_string out "NRst)\n"
+     | Rst (e1, e2) ->
+        output_string out "Sreg (mk_freg ("; output_string out ((r.rid)^" "); pp_type out (r.rtype); output_string out " "; pp_expr out (r.clock); output_string out " "; output_string out "(Rst "; pp_expr out e1; output_string out " "; pp_expr out e2; output_string out ")\n")
+  | Snode (v, e) -> output_string out "(Snode "; output_string out (v^" "); pp_expr out e; output_string out ")\n"
   | _ -> output_string out ""
                  
           
 let pp_module out fmod =
   match fmod with
-  | FInmod (v, pl, sl) -> output_string out "(FInmod "; output_string out (v^" "); pp_ports out pl; pp_statements out sl; output_string out ")\n"
+  | FInmod (v, pl, sl) -> output_string out "(FInmod "; output_string out (v^"\n"); pp_ports out pl; pp_statements out sl; output_string out ")\n"
   | _ -> output_string out "\n"
           
 let pp_modules out fmod = List.iter (fun c -> pp_module out c; output_string out "") fmod
 
 let pp_fcircuit out fc =
   match fc with
-  | (v, fmod) -> output_string out "(FCircuit "; output_string out (v^" "); pp_modules out fmod; output_string out ")"
+  | (v, fmod) -> output_string out "(FCircuit "; output_string out (v^"\n"); pp_modules out fmod; output_string out ")\n"
 
 let pp_file out fc = pp_fcircuit out fc
