src/Env.v
@@ -1,0 +1,465 @@
+From Coq Require Import FunInd FMaps FMapAVL OrderedType.
+From mathcomp Require Import ssreflect ssrbool ssrnat ssrint eqtype seq.
+From simplssrlib Require Import Types SsrOrder FSets FMaps Tactics Var Store.
+From nbits Require Import NBits.
+
+Set Implicit Arguments.
+Unset Strict Implicit.
+Import Prenex Implicits.
+
+  (****** Types Environment ******)
+
+  (****** Ground Types ******)
+
+  From Coq Require Import ZArith.
+
+  Inductive fgtyp : Set :=
+    Fuint : nat -> fgtyp
+  | Fsint : nat -> fgtyp
+  | Fclock.
+  (* | Fanalog : nat -> fgtyp *) (* TBD, HiFirrtl *)
+  (* | Fvector : fgtyp -> nat -> fgtyp *) (* TBD, HiFirrtl *)
+
+  (* Size of types *)
+
+  Definition sizeof_fgtyp (t : fgtyp) : nat :=
+    match t with
+    | Fuint w => w
+    | Fsint w => w
+    (* | Fanalog w => w *)
+    | Fclock => 1
+    end.
+
+  
+  (* Equality of types *)
+
+  Lemma fgtyp_eq_dec (x y : fgtyp) : {x = y} + {x <> y}.
+  Proof.
+    destruct x; destruct y; try (intros; right; move=> []; discriminate).
+    - intros; case: (Nat.eq_dec n n0) => H.
+      + left; rewrite H; reflexivity.
+      + right; move=> []; auto.
+    - intros; case: (Nat.eq_dec n n0) => H.
+      + left; rewrite H; reflexivity.
+      + right; move=> []; auto.
+    (* - intros; case: (Nat.eq_dec n n0) => H. *)
+    (*   + left; rewrite H; reflexivity. *)
+    (*   + right; move=> []; auto. *)
+    - left; done.
+  Qed.
+
+  Definition fgtyp_eqn (x y : fgtyp) : bool :=
+    match x, y with
+    | Fuint wx, Fuint wy => wx == wy
+    | Fsint wx, Fsint wy => wx == wy
+    (* | Fanalog wx, Fanalog wy => wx == wy *)
+    | Fclock, Fclock => true
+    | _, _ => false
+    end.
+
+  Notation "x =? y" := (fgtyp_eqn x y).
+
+  Lemma fgtyp_eqn_refl (x : fgtyp) : x =? x.
+  Proof.
+    destruct x; try (exact: eqxx).
+    - done.
+  Qed.
+
+  Lemma fgtyp_eqn_eq (x y : fgtyp) : x =? y <-> x = y.
+  Proof.
+    split; first (destruct x; destruct y; move=> /= H);
+      try (discriminate|| rewrite (eqP H); reflexivity).
+    - done.
+    - move=> ->. exact: fgtyp_eqn_refl.
+  Qed.
+
+  Lemma fgtyp_eqn_sym (x y : fgtyp) : x =? y -> y =? x.
+  Proof.
+    move/fgtyp_eqn_eq => H. apply/fgtyp_eqn_eq. symmetry. assumption.
+  Qed.
+
+  Lemma fgtyp_eqn_trans (x y z : fgtyp) : x =? y -> y =? z -> x =? z.
+  Proof.
+    move/fgtyp_eqn_eq => Hxy. move/fgtyp_eqn_eq => Hyz. apply/fgtyp_eqn_eq.
+    rewrite Hxy. assumption.
+  Qed.
+
+  Instance fgtyp_eqn_Reflexive : Reflexive (@fgtyp_eqn) := @fgtyp_eqn_refl.
+  Instance fgtyp_eqn_Symmetric : Symmetric (@fgtyp_eqn) := @fgtyp_eqn_sym.
+  Instance fgtyp_eqn_Transitive : Transitive (@fgtyp_eqn) := @fgtyp_eqn_trans.
+  Instance fgtyp_eqn_Equivalence : Equivalence (@fgtyp_eqn) :=
+    { Equivalence_Reflexive := fgtyp_eqn_Reflexive;
+      Equivalence_Symmetric := fgtyp_eqn_Symmetric;
+      Equivalence_Transitive := fgtyp_eqn_Transitive }.
+
+  Lemma fgtyp_eqP : forall (x y : fgtyp), reflect (x = y) (x =? y).
+  Proof.
+    move=> x y. case H: (x =? y).
+    - apply: ReflectT. apply/fgtyp_eqn_eq. assumption.
+    - apply: ReflectF. move=> Heq. move/fgtyp_eqn_eq: Heq => Heq. rewrite Heq in H.
+      discriminate.
+  Qed.
+
+  Definition fgtyp_eqMixin := EqMixin fgtyp_eqP.
+  Canonical fgtyp_eqType := Eval hnf in EqType fgtyp fgtyp_eqMixin.
+
+
+  (*Delimit Scope fgtyp_scope with fgtyp.*)
+
+(* A typing environment is a map from a variable to its type *)
+
+Module Type TypEnv <: SsrFMap.
+
+  Include SsrFMap.
+
+  Definition env : Type := t fgtyp.
+
+  (* The default type of a variable not in the typing environment *)
+  Parameter deftyp : fgtyp.
+
+  (* Find the type of a variable in a typing environment.
+     If a variable is not in the typing environment, return the default type. *)
+  Parameter vtyp : SE.t -> env -> fgtyp.
+
+  (* Return the size of a variable in a typing environment.
+     If a variable is not in the typing environment, return the size of the
+     default type. *)
+  Parameter vsize : SE.t -> env -> nat.
+
+  Axiom find_some_vtyp :
+    forall {x : SE.t} {ty : fgtyp} {e : env}, find x e = Some ty -> vtyp x e = ty.
+  Axiom find_none_vtyp :
+    forall {x : SE.t} {e : env}, find x e = None -> vtyp x e = deftyp.
+  Axiom vtyp_find :
+    forall {x : SE.t} {ty : fgtyp} {e : env},
+      (vtyp x e == ty) = (find x e == Some ty) || ((find x e == None) && (ty == deftyp)).
+  Axiom vtyp_add_eq :
+    forall {x y : SE.t} {ty : fgtyp} {e : env}, x == y -> vtyp x (add y ty e) = ty.
+  Axiom vtyp_add_neq :
+    forall {x y : SE.t} {ty : fgtyp} {e : env},
+      x != y -> vtyp x (add y ty e) = vtyp x e.
+  Axiom vsize_add_eq :
+    forall {x y : SE.t} {ty : fgtyp} {e : env},
+      x == y -> vsize x (add y ty e) = sizeof_fgtyp ty.
+  Axiom vsize_add_neq :
+    forall {x y : SE.t} {ty : fgtyp} {e : env},
+      x != y -> vsize x (add y ty e) = vsize x e.
+  Axiom not_mem_vtyp :
+    forall {v : SE.t} {e : env}, ~~ mem v e -> vtyp v e = deftyp.
+  Axiom vtyp_vsize :
+    forall {x : SE.t} {e : env} {ty : fgtyp},
+      vtyp x e = ty -> vsize x e = sizeof_fgtyp ty.
+
+End TypEnv.
+
+Module MakeTypEnv (V : SsrOrder) (VM : SsrFMap with Module SE := V) <:
+  TypEnv with Module SE := V.
+
+  Include VM.
+  Module Lemmas := FMapLemmas VM.
+
+  Definition env : Type := t fgtyp.
+
+  (* The default type of a variable not in the typing environment *)
+  Definition deftyp : fgtyp := Fuint 0.
+
+  (* Find the type of a variable in a typing environment.
+     If a variable is not in the typing environment, return the default type. *)
+  Definition vtyp (v : V.t) (e : env) : fgtyp :=
+    match VM.find v e with
+    | None => deftyp
+    | Some ty => ty
+    end.
+
+  (* Return the size of a variable in a typing environment.
+     If a variable is not in the typing environment, return the size of the
+     default type. *)
+  Definition vsize (v : V.t) (e : env) : nat := sizeof_fgtyp (vtyp v e).
+
+  Lemma find_some_vtyp {x ty e} : find x e = Some ty -> vtyp x e = ty.
+  Proof. move=> H. rewrite /vtyp H. reflexivity. Qed.
+
+  Lemma find_none_vtyp {x e} : find x e = None -> vtyp x e = deftyp.
+  Proof. move=> H. rewrite /vtyp H. reflexivity. Qed.
+
+  Lemma vtyp_find {x ty e} :
+    (vtyp x e == ty) = (find x e == Some ty) || ((find x e == None) && (ty == deftyp)).
+  Proof.
+    dcase (find x e); case.
+    - move=> a Hfind. rewrite (find_some_vtyp Hfind) /= orbF. case Heq: (a == ty).
+      + by rewrite (eqP Heq) eqxx.
+      + symmetry. apply/eqP => H. case: H => H. rewrite H eqxx in Heq. discriminate.
+    - move=> Hnone. rewrite (find_none_vtyp Hnone) eqxx /=. rewrite eq_sym.
+      reflexivity.
+  Qed.
+
+  Lemma vtyp_add_eq {x y ty e} : x == y -> vtyp x (add y ty e) = ty.
+  Proof. rewrite /vtyp /add => H. by rewrite (Lemmas.find_add_eq H). Qed.
+
+  Lemma vtyp_add_neq {x y ty e} : x != y -> vtyp x (add y ty e) = vtyp x e.
+  Proof.
+    move/negP=> Hxy. rewrite /vtyp /add. by rewrite (Lemmas.find_add_neq Hxy).
+  Qed.
+
+  Lemma vsize_add_eq {x y ty e} : x == y -> vsize x (add y ty e) = sizeof_fgtyp ty.
+  Proof. rewrite /vsize=> H. by rewrite (vtyp_add_eq H). Qed.
+
+  Lemma vsize_add_neq {x y ty e} : x != y -> vsize x (add y ty e) = vsize x e.
+  Proof. rewrite /vsize => H. by rewrite (vtyp_add_neq H). Qed.
+
+  Lemma not_mem_vtyp v e : ~~ mem v e -> vtyp v e = deftyp.
+  Proof. rewrite /vtyp => H. by rewrite Lemmas.not_mem_find_none. Qed.
+
+  Lemma vtyp_vsize x e ty : vtyp x e = ty -> vsize x e = sizeof_fgtyp ty.
+  Proof. rewrite /vsize /vtyp. move=> ->. reflexivity. Qed.
+
+End MakeTypEnv.
+
+Module TE <: TypEnv := MakeTypEnv VarOrder VM.
+
+(* TBD *)
+(* Variable structure : Type. *)
+
+(* Module Type StrStore (V : SsrOrder) (TE : TypEnv with Module SE := V). *)
+(*   Module Lemmas := FMapLemmas TE. *)
+
+(*   Local Notation var := V.t. *)
+(*   Local Notation value := structure. *)
+
+(*   Parameter t : Type. *)
+(*   Parameter acc : var -> t -> value. *)
+(*   Parameter upd : var -> value -> t -> t. *)
+(*   Parameter upd2 : var -> value -> var -> value -> t -> t. *)
+  
+(* End StrStore. *)
+
+(* Module MakeStrStore (V : SsrOrder) (TE : TypEnv with Module SE := V) <: *)
+(*   StrStore V TE. *)
+(*   Module Lemmas := FMapLemmas TE. *)
+
+(* End MakeStrStore. *)
+
+(* Module StrStore := MakeStrStore VarOrder TE. *)
+
+Module Type ValStore (V : SsrOrder) (TE : TypEnv with Module SE := V).
+  Module Lemmas := FMapLemmas TE.
+
+  Local Notation var := V.t.
+  Local Notation value := bits.
+
+  Parameter t : Type.
+  Parameter acc : var -> t -> value.
+  Parameter upd : var -> value -> t -> t.
+  Parameter upd2 : var -> value -> var -> value -> t -> t.
+    Parameter acc_upd_eq : forall {x y v s}, x == y -> acc x (upd y v s) = v.
+  Parameter acc_upd_neq : forall {x y v s}, x != y -> acc x (upd y v s) = acc x s.
+  Parameter acc_upd2_eq1 :
+    forall {x y1 v1 y2 v2 s},
+      x == y1 -> x != y2 -> acc x (upd2 y1 v1 y2 v2 s) = v1.
+  Parameter acc_upd2_eq2 :
+    forall {x y1 v1 y2 v2 s},
+      x == y2 -> acc x (upd2 y1 v1 y2 v2 s) = v2.
+  Parameter acc_upd2_neq :
+    forall {x y1 v1 y2 v2 s},
+      x != y1 -> x != y2 -> acc x (upd2 y1 v1 y2 v2 s) = acc x s.
+  Parameter Upd : var -> value -> t -> t -> Prop.
+  Definition Upd2 x1 v1 x2 v2 (s1 s2 : t) : Prop :=
+    forall y, acc y s2 = acc y (upd x2 v2 (upd x1 v1 s1)).
+  Parameter Equal : t -> t -> Prop.
+  Parameter Upd_upd : forall x v s, Upd x v s (upd x v s).
+  Parameter Upd2_upd :
+    forall x1 v1 x2 v2 s, Upd2 x1 v1 x2 v2 s (upd x2 v2 (upd x1 v1 s)).
+  Parameter Upd2_upd2 : forall x1 v1 x2 v2 s, Upd2 x1 v1 x2 v2 s (upd2 x1 v1 x2 v2 s).
+  Parameter acc_Upd_eq : forall x y v s1 s2, x == y -> Upd y v s1 s2 -> acc x s2 = v.
+  Parameter acc_Upd_neq :
+    forall x y v s1 s2, x != y -> Upd y v s1 s2 -> acc x s2 = acc x s1.
+  Parameter acc_Upd2_eq1 :
+    forall x y1 v1 y2 v2 s1 s2,
+      x == y1 -> x != y2 -> Upd2 y1 v1 y2 v2 s1 s2 -> acc x s2 = v1.
+  Parameter acc_Upd2_eq2 :
+    forall x y1 v1 y2 v2 s1 s2, x == y2 -> Upd2 y1 v1 y2 v2 s1 s2 -> acc x s2 = v2.
+  Parameter acc_Upd2_neq :
+    forall x y1 v1 y2 v2 s1 s2,
+      x != y1 -> x != y2 -> Upd2 y1 v1 y2 v2 s1 s2 -> acc x s2 = acc x s1.
+  Parameter Equal_def :
+    forall s1 s2,
+      Equal s1 s2 <-> (forall v, acc v s1 = acc v s2).
+  Parameter Equal_refl : forall s, Equal s s.
+  Parameter Equal_sym : forall s1 s2, Equal s1 s2 -> Equal s2 s1.
+  Parameter Equal_trans : forall s1 s2 s3, Equal s1 s2 -> Equal s2 s3 -> Equal s1 s3.
+  Parameter Equal_ST : RelationClasses.Equivalence Equal.
+  Parameter Equal_upd_Equal :
+    forall v e s1 s2, Equal s1 s2 -> Equal (upd v e s1) (upd v e s2).
+  Parameter Equal_Upd_Equal :
+    forall v e s1 s2 s3 s4,
+      Upd v e s1 s2 -> Upd v e s3 s4 -> Equal s1 s3 -> Equal s2 s4.
+  Parameter Upd_pred_Equal :
+    forall v e s1 s2 s, Upd v e s1 s2 -> Equal s1 s -> Upd v e s s2.
+  Parameter Upd_succ_Equal :
+    forall v e s1 s2 s, Upd v e s1 s2 -> Equal s2 s -> Upd v e s1 s.
+
+  Parameter conform : t -> TE.env -> Prop.
+  Parameter conform_def :
+    forall (s : t) (E : TE.env),
+      (forall (v : V.t), TE.mem v E -> TE.vsize v E = size (acc v s)) ->
+      conform s E.
+  Parameter conform_mem :
+    forall v s te, conform s te -> TE.mem v te -> TE.vsize v te = size (acc v s).
+  Parameter conform_Upd :
+    forall x ty v s1 s2 te,
+      sizeof_fgtyp ty = size v -> Upd x v s1 s2 -> conform s1 te ->
+      conform s2 (TE.add x ty te).
+  Parameter conform_Upd2 :
+    forall te s1 s2 ty1 ty2 x1 x2 v1 v2,
+      x1 != x2 -> sizeof_fgtyp ty1 = size v1 -> sizeof_fgtyp ty2 = size v2 ->
+      Upd2 x2 v2 x1 v1 s1 s2 -> conform s1 te ->
+      conform s2 (TE.add x1 ty1 (TE.add x2 ty2 te)).
+  Parameter conform_upd :
+    forall x ty v s te,
+      sizeof_fgtyp ty = size v -> conform s te -> conform (upd x v s) (TE.add x ty te).
+  Parameter conform_upd2 :
+    forall te s ty1 ty2 x1 x2 v1 v2,
+      x1 != x2 -> sizeof_fgtyp ty1 = size v1 -> sizeof_fgtyp ty2 = size v2 ->
+      conform s te ->
+      conform (upd2 x2 v2 x1 v1 s) (TE.add x1 ty1 (TE.add x2 ty2 te)).
+  Parameter conform_add_not_mem :
+    forall E s x ty,
+      conform s (TE.add x ty E) -> ~~ TE.mem x E -> conform s E.
+  Parameter conform_submap :
+    forall E1 E2 s,
+      Lemmas.submap E1 E2 -> conform s E2 -> conform s E1.
+  Parameter conform_equal :
+    forall E1 E2 s,
+      TE.Equal E1 E2 -> conform s E1 <-> conform s E2.
+  Parameter equal_conform :
+    forall E s1 s2,
+      Equal s1 s2 -> conform s1 E <-> conform s2 E.
+End ValStore.
+
+Module BValueType <: HasDefaultTyp.
+  Definition t : Type := bits.
+  Definition default : t := [::b0].
+End BValueType.
+
+Module MakeValStore (V : SsrOrder) (TE : TypEnv with Module SE := V) <:
+  ValStore V TE.
+
+  Include MakeTStoreMap V BValueType. 
+  Module Lemmas := FMapLemmas TE.
+
+  (* A store conforms to a typing environment if for every variable in the typing
+     environment, the size of its type in the typing environment is the same as
+     the size of its value in the store *)
+  Definition conform (s : t) (te : TE.env) : Prop :=
+    forall (v : V.t),
+      TE.mem v te -> TE.vsize v te = size (acc v s).
+
+  Lemma conform_def :
+    forall (s : t) (E : TE.env),
+      (forall (v : V.t), TE.mem v E -> TE.vsize v E = size (acc v s)) ->
+      conform s E.
+  Proof. move=> s E H. assumption. Qed.
+
+  Lemma conform_mem v s te :
+    conform s te -> TE.mem v te -> TE.vsize v te = size (acc v s).
+  Proof. move=> H1 H2; exact: (H1 _ H2). Qed.
+
+  Lemma conform_Upd x ty v s1 s2 te :
+    sizeof_fgtyp ty = size v -> Upd x v s1 s2 -> conform s1 te ->
+    conform s2 (TE.add x ty te).
+  Proof.
+    move=> Hs Hupd Hcon y. case Hyx: (y == x).
+    - by rewrite (TE.vsize_add_eq Hyx) (acc_Upd_eq Hyx Hupd).
+    - move/negP: Hyx => Hyx. rewrite (Lemmas.mem_add_neq Hyx) => Hmem.
+      move/negP: Hyx => Hyx. rewrite (acc_Upd_neq Hyx Hupd) (TE.vsize_add_neq Hyx).
+      exact: (Hcon _ Hmem).
+  Qed.
+
+  Lemma conform_Upd2 te s1 s2 ty1 ty2 x1 x2 v1 v2 :
+    x1 != x2 -> sizeof_fgtyp ty1 = size v1 -> sizeof_fgtyp ty2 = size v2 ->
+    Upd2 x2 v2 x1 v1 s1 s2 -> conform s1 te ->
+    conform s2 (TE.add x1 ty1 (TE.add x2 ty2 te)).
+  Proof.
+    move => Hneq Hty1 Hty2 HUpd2 Hcon y Hmem .
+    case Heq1 : (y == x1); case Heq2 : (y == x2) .
+    - rewrite -(eqP Heq1) -(eqP Heq2) in Hneq . move : Hneq => /eqP // .
+    - rewrite (acc_Upd2_eq2 Heq1 HUpd2) (TE.vsize_add_eq Heq1) // .
+    - move/idP/negP: Heq1 => Hneq1.
+      rewrite (acc_Upd2_eq1 Heq2 Hneq1 HUpd2)
+              (TE.vsize_add_neq Hneq1) (TE.vsize_add_eq Heq2) // .
+    - move/idP/negP: Heq1 => Hneq1.
+      move/idP/negP: Heq2 => Hneq2.
+      rewrite (acc_Upd2_neq Hneq2 Hneq1 HUpd2)
+              (TE.vsize_add_neq Hneq1) (TE.vsize_add_neq Hneq2) Hcon // .
+      move/negP: Hneq1 => Hneq1. move/negP: Hneq2 => Hneq2.
+      rewrite (Lemmas.mem_add_neq Hneq1) (Lemmas.mem_add_neq Hneq2) in Hmem.
+      assumption.
+  Qed.
+
+  Lemma conform_upd x ty v s te :
+    sizeof_fgtyp ty = size v ->
+    conform s te -> conform (upd x v s) (TE.add x ty te).
+  Proof. move=> Hs Hcon. exact: (conform_Upd Hs (Upd_upd x v s) Hcon). Qed.
+
+  Lemma conform_upd2 te s ty1 ty2 x1 x2 v1 v2 :
+    x1 != x2 -> sizeof_fgtyp ty1 = size v1 -> sizeof_fgtyp ty2 = size v2 ->
+    conform s te ->
+    conform (upd2 x2 v2 x1 v1 s) (TE.add x1 ty1 (TE.add x2 ty2 te)).
+  Proof.
+    move=> Hne Hs1 Hs2 Hcon.
+    exact: (conform_Upd2 Hne Hs1 Hs2 (Upd2_upd2 x2 v2 x1 v1 s) Hcon).
+  Qed.
+
+  Lemma conform_add_not_mem E s x ty :
+    conform s (TE.add x ty E) -> ~~ TE.mem x E -> conform s E.
+  Proof.
+    move=> Hco Hmem y Hmemy. move: (Hco y). rewrite Lemmas.OP.P.F.add_b Hmemy orbT.
+    move=> <-; last by exact: is_true_true. case Hyx: (y == x).
+    - rewrite (eqP Hyx) in Hmemy. rewrite Hmemy in Hmem. discriminate.
+    - move/idP/negP: Hyx => Hyx. rewrite (TE.vsize_add_neq Hyx). reflexivity.
+  Qed.
+
+  Lemma conform_submap E1 E2 s :
+    Lemmas.submap E1 E2 -> conform s E2 -> conform s E1.
+  Proof.
+    move=> Hsubm Hco x Hmem1. move: (Lemmas.submap_mem Hsubm Hmem1) => Hmem2.
+    move: (Lemmas.mem_find_some Hmem1) => [ty Hfind1].
+    move: (Hsubm x ty Hfind1) => Hfind2. move: (TE.find_some_vtyp Hfind1) => Hty1.
+     move: (TE.find_some_vtyp Hfind2) => Hty2. rewrite -(Hco _ Hmem2).
+    rewrite (TE.vtyp_vsize Hty1) (TE.vtyp_vsize Hty2). reflexivity.
+  Qed.
+
+  Lemma conform_equal E1 E2 s :
+    TE.Equal E1 E2 -> conform s E1 <-> conform s E2.
+  Proof.
+    move=> Heq. move: (Lemmas.Equal_submap Heq) => H12.
+    move: (Lemmas.Equal_sym Heq) => {Heq} Heq.
+    move: (Lemmas.Equal_submap Heq) => H21. split.
+    - exact: (conform_submap H21).
+    - exact: (conform_submap H12).
+  Qed.
+
+  Lemma equal_conform E s1 s2 :
+    Equal s1 s2 -> conform s1 E <-> conform s2 E.
+  Proof.
+    move=> Heq. split.
+    - move=> H1. apply: conform_def. move=> v Hmem.
+      rewrite (conform_mem H1 Hmem). rewrite (Heq v). reflexivity.
+    - move=> H2. apply: conform_def. move=> v Hmem.
+      rewrite (conform_mem H2 Hmem). rewrite (Heq v). reflexivity.
+  Qed.
+
+End MakeValStore.
+
+Module Store := MakeValStore VarOrder TE.
+
+Section State.
+  Variable t : Type.
+  Inductive state : Type :=
+  | OK of t
+  | ERR.
+End State.
+
+Module State.
+  Definition t : Type := state Store.t.
+End State.
